CFG.dfy
@@ -1,0 +1,24 @@
+include "Definitions.dfy"
+include "Util.dfy"
+
+// Label Definition from AST of the Statement:
+newtype Branch = b: int | 1 <= b <= 2
+type Label = seq<Branch>
+
+// CFG Definitions:
+datatype CFGNode = Node(l:Label) | Entry | Exit
+type CFGEdge = (CFGNode, CFGNode)
+type CFG = (set<CFGNode>, set<CFGEdge>)
+
+method ComputeCFG(S: Statement) returns (N: set<CFGNode>, E: set<CFGEdge>)
+{
+	
+}
+
+function FindSubstatement(S: Statement, l: Label) : Statement
+
+function UsedVars(S: Statement, l: Label) : set<Variable>
+	// call FindSubstatement
+
+function DefinedVars(S: Statement, l: Label) : set<Variable>
+	// call FindSubstatement
