Sliding-11.1-11.2.dfy
@@ -11,7 +11,6 @@ requires Vr <= V
 requires Valid(S)
 ensures Valid(Scov)
 {
-	//var fVr := Fresh(Vr, V+glob(S));
 	var freshV := new Fresh();
 	assert forall v :: v in Vr ==> v !in freshV.range by {
 		assert freshV.range == {};
@@ -20,8 +19,8 @@ ensures Valid(Scov)
 	assert forall v :: v in glob(S) ==> v !in fVr by {
 		assert forall v :: v in glob(S) ==> v in fSetToSeq(glob(S));
 	}
-	var S' := ComputeCoSlice(S, V, Vr, fVr/*, freshV*/);
-	assert forall v :: v in glob(S') ==> v !in Vr;
+	var S' := ComputeCoSlice(S, V, Vr, fVr);
+	assert mutuallyDisjoint([Vr, fSetToSeq(glob(S'))]);
 
 	Scov := FinalUseSubstitution(S', fVr, Vr);
 }
@@ -39,70 +38,82 @@ lemma {:verify true} Refinement11_1(
 	icoV: seq<Variable>,
 	fVr: seq<Variable>,
 	fVnr: seq<Variable>)
+requires |Vr|==|fVr|
+requires |Vnr|==|fVnr|
+requires |iVr|==|Vr|
+requires |iVnr|==|Vnr|
+requires |icoV|==|coV|
+requires mutuallyDisjoint([fVr, fSetToSeq(glob(S))]);
+requires mutuallyDisjoint([Vr,fVr])
+requires mutuallyDisjoint([Vnr,fVnr])
 requires Valid(S)
 requires Valid(Sv)
 requires Valid(Scov)
+requires Core(Scov)
+requires mutuallyDisjoint([Vr,Vnr,coV])
+requires def(S) == setOf(Vr+Vnr+coV)
 requires 
 	var S' := Live(Vr+Vnr, S);
 	var Sv' := Live(Vr+Vnr, Sv);
-	Refinment(S', Sv');
-requires mutuallyDisjoint([Vr,Vnr,coV])
-requires mutuallyDisjoint([iVr,iVnr,icoV,fVr,fVnr])
+	Refinement(S', Sv');
+requires 
+	var Scov' := Live(coV, Scov);
+	var S' := FinalUseSubstitution(S, Vr, fVr);
+	Refinement(Live(coV, S'), Scov');
 requires def(Sv) <= def(S);
 requires def(Scov) <= def(S);
-requires uniqueness(Vr);
-requires uniqueness(Vnr);
-requires uniqueness(iVr);
-requires uniqueness(iVnr);
-requires uniqueness(fVr);
-requires uniqueness(fVnr);
-requires uniqueness(coV);
-requires uniqueness(icoV);
-requires |Vr| == |fVr|
-requires |Vnr| == |fVnr|
-requires |iVr| == |Vr|
-requires |iVnr| == |Vnr|
-requires |icoV| == |coV|
-requires forall v :: v in Vr ==> v !in fVr
-requires forall v :: v in fVr ==> v !in glob(S)
+requires mutuallyDisjoint([iVr,iVnr,icoV,fVr,fVnr])
+requires mutuallyDisjoint([iVr+iVnr+icoV+fVr+fVnr, fSetToSeq(glob(S))])
 ensures 
-	var Vr1 := setOf(Vr)*input(Scov);
-	var Vr2 := setOf(Vr)*(def(Scov)-input(Scov));
+	var Vr1 := seqConjunction(Vr, fSetToSeq(input(Scov)));
+	var Vr2 := seqConjunction(Vr, fSetToSeq(def(Scov)-input(Scov)));
 	var Vr3 := seqSubtraction(Vr, fSetToSeq(glob(Scov)));
-	var iVr1 := setOf(iVr)*input(Scov);
-	var iVr2 := setOf(iVr)*(def(Scov)-input(Scov));
-	var iVr3 := setOf(iVr)-glob(Scov);
-	var fVr1 := setOf(fVr)*input(Scov);
-	var fVr2 := setOf(fVr)*(def(Scov)-input(Scov));
-	var fVr3 := seqSubtraction(fVr,fSetToSeq(glob(Scov)));
+	var iVr1 := corresponding(Vr, iVr, setOf(Vr1));//setOf(iVr)*input(Scov);
+	var iVr2 := corresponding(Vr, iVr, setOf(Vr2));//setOf(iVr)*(def(Scov)-input(Scov));
+	var iVr3 := corresponding(Vr, iVr, setOf(Vr3));//setOf(iVr)-glob(Scov);
+	var fVr1 := corresponding(Vr, fVr, setOf(Vr1));//setOf(fVr)*input(Scov);
+	var fVr2 := corresponding(Vr, fVr, setOf(Vr2));//setOf(fVr)*(def(Scov)-input(Scov));
+	var fVr3 := corresponding(Vr, fVr, setOf(Vr3));//seqSubtraction(fVr,fSetToSeq(glob(Scov)));
 
-	var Vnr1 := setOf(Vnr)*input(Scov);
-	var Vnr2 := setOf(Vnr)*(def(Scov)-input(Scov));
-	var Vnr3 := setOf(Vnr)-glob(Scov);
-	var iVnr1 := setOf(iVnr)*input(Scov);
-	var iVnr2 := setOf(iVnr)*(def(Scov)-input(Scov));
-	var iVnr3 := setOf(iVnr)-glob(Scov);
-	var fVnr1 := setOf(fVnr)*input(Scov);
-	var fVnr2 := setOf(fVnr)*(def(Scov)-input(Scov));
-	var fVnr3 := setOf(fVnr)-glob(Scov);
+	var Vnr1 := seqConjunction(Vnr, fSetToSeq(input(Scov)));
+	var Vnr2 := seqConjunction(Vnr, fSetToSeq(def(Scov)-input(Scov)));
+	var Vnr3 := seqSubtraction(Vnr, fSetToSeq(glob(Scov)));
+	var iVnr1 := corresponding(Vnr, iVnr, setOf(Vnr1));//setOf(iVnr)*input(Scov);
+	var iVnr2 := corresponding(Vnr, iVnr, setOf(Vnr2));//setOf(iVnr)*(def(Scov)-input(Scov));
+	var iVnr3 := corresponding(Vnr, iVnr, setOf(Vnr3));//setOf(iVnr)-glob(Scov);
+	var fVnr1 := corresponding(Vnr, fVnr, setOf(Vnr1));//setOf(fVnr)*input(Scov);
+	var fVnr2 := corresponding(Vnr, fVnr, setOf(Vnr2));//setOf(fVnr)*(def(Scov)-input(Scov));
+	var fVnr3 := corresponding(Vnr, fVnr, setOf(Vnr3));//setOf(fVnr)-glob(Scov);
 	
-	var coV11 := setOf(coV)*def(Sv)*input(Scov);
-	var coV12 := setOf(coV)*(input(Scov)-def(Sv));
-	var coV2 := setOf(coV) - input(Scov);
-	var icoV11 := setOf(icoV)*def(Sv)*input(Scov);
-	var icoV12 := setOf(icoV)*(input(Scov)-def(Sv));
-	var icoV2 := setOf(icoV) - input(Scov);
+	var coV11 := seqConjunction(coV, fSetToSeq(def(Sv)*input(Scov)));
+	var coV12 := seqConjunction(coV, fSetToSeq(input(Scov)-def(Sv)));
+	var coV2 := seqSubtraction(coV, fSetToSeq(input(Scov)));
+	var icoV11 := corresponding(coV, icoV, setOf(coV11));//setOf(icoV)*def(Sv)*input(Scov);
+	var icoV12 := corresponding(coV, icoV, setOf(coV12));//setOf(icoV)*(input(Scov)-def(Sv));
+	var icoV2 := corresponding(coV, icoV, setOf(coV2));//setOf(icoV) - input(Scov);
 
-	
-	assume |Vr3| == |fVr3|;
-	var Scovsub := FinalUseSubstitution(Scov, Vr3, fVr3);
-	assert def(Sv) <= def(S);
-	assert def(Scov) <= def(S);
+	var sVr := setOf(Vr);
+	var sfVr := setOf(fVr);
+	var sVr3 := setOf(Vr3);
+	var sfVr3 := setOf(fVr3);
 
-	var vars : seq<Variable> := fSetToSeq(Vr1+Vnr1+coV11);
-	var ivars : seq<Variable> := fSetToSeq(iVr1+iVnr1+icoV11);
-	var varsb : seq<Variable> := fSetToSeq(Vr1+Vr2+Vnr1+Vnr2);
-	var fvars : seq<Variable> := fSetToSeq(fVr1+fVr2+fVnr1+fVnr2);
+
+	assert |fVr3| == |Vr3| by {
+		assume |sVr3| == |Vr3|;
+	}
+	assert mutuallyDisjoint([Vr3, fVr3]) by {
+		assert mutuallyDisjoint([Vr, fVr]);
+		assert sfVr3 <= sfVr;
+		assert sVr3 <= sVr;
+		assume sVr3 !! sfVr3;//<<<
+	}
+	assume mutuallyDisjoint([Vr3, fSetToSeq(allVars(Scov))]);//<<<
+	var Scovsub := substitute(Scov, fVr3, Vr3);
+
+	var vars : seq<Variable> := Vr1+Vnr1+coV11;
+	var ivars : seq<Variable> := iVr1+iVnr1+icoV11;
+	var varsb : seq<Variable> := Vr1+Vr2+Vnr1+Vnr2;
+	var fvars : seq<Variable> := fVr1+fVr2+fVnr1+fVnr2;
 	var varse := seqVarToSeqExpr(vars);
 	var ivarse := seqVarToSeqExpr(ivars);
 	var varsbe := seqVarToSeqExpr(varsb);
@@ -114,24 +125,8 @@ ensures
 					SeqComp(Sv, 
 						SeqComp(Assignment(fvars, varsbe),
 							SeqComp(Assignment(vars, ivarse),
-								SeqComp(Scov, Assignment(varsb, fvarse)))))));
+								SeqComp(Scovsub, Assignment(varsb, fvarse)))))));
 
-/*	assume Valid(result);
-	calc {
-		|ivars|;
-		== 
-		|varse|;
-		== 
-		|vars|;
-	}
-	calc {
-		|varsbe|; 
-		== 
-		|varsb|;
-		== 
-		|Vr1|+|Vr2|+|Vnr1|+|Vnr2|;
-		==
-		|fvars|;
-	}*/
+	assert Valid(result);
 	Refinement(S, result)
 
